killed many frame_admits with frame_unrelated; still a few remain

src/tls/TLS.fst
@@ -19,267 +19,11 @@ open TLSInfo
 open Range
 open StatefulLHAE // via its interface
 open Handshake    // via its interface
+open Connection
+
+
 
 // using also Alert, Range, DataStream, TLSFragment, Record
-
-// internal state machine (one for reading, one for writing; a bit much)
-// TODO make it private?
-// TODO write invariant, to cut out cases in code
-// e.g. , reading, and writing transitions are tighly related
-// TODO recheck large logical invariants GState in Dispatch.fs7
-
-// private //TODO: restore this qualifier; NS:commenting for now
-type dispatch =
-  | Init
-  | FirstHandshake of ProtocolVersion (* bound by ServerHello *)
-  | Finishing
-  | Finished
-  | Open
-  | Closing of ProtocolVersion * string (* write-only, while sending a fatal alert *)
-  | Closed
- 
-type connection = | C:
-  #region: rid ->
-  peer:   rid{disjoint region peer} ->
-  hs:      hs { extends (HS.region hs) region /\ extends (HS.peer hs) peer } (* providing role, config, and uid *) ->
-  alert:   Alert.state  { extends (Alert.State.region alert) region /\ HS.region hs <> Alert.State.region alert } (* review *) ->
-  tcp:     networkStream ->
-  reading: rref region dispatch ->
-  writing: rref region dispatch ->
-  connection
-
-let c_role c   = c.hs.r
-let c_id c     = c.hs.id
-let c_cfg c    = c.hs.cfg
-let c_resume c = c.hs.resume
-let c_log c    = c.hs.log
-
-
-(*** top-level invariant (TBC) ***) 
-
-// we'll rely on the invariant to show we picked the correct index
-
-opaque type Seq_forall (#a:Type) (p: a -> Type) (s:seq a) =
-  forall (j: nat { j < Seq.length s }).{:pattern (Seq.index s j)} p (Seq.index s j)
-
-let test_1 (p:nat -> Type) (s:seq nat { Seq_forall p s }) = assert(p 12 ==> Seq_forall p (snoc s 12))
-let test_2 (p:nat -> Type) (s:seq nat { Seq_forall p s }) (j:nat { j < Seq.length s }) =  let x = Seq.index s j in assert(p x)
-//let test_3 (p:nat -> Type) (s:seq nat { Seq_forall p s }) x = assert(SeqProperties.mem x s ==> p x)
-
-
-(* usage? how to prove this lemma?  val exercise_seq_forall: #a:Type
--> p: (a -> Type) -> s:seq a -> x: a -> Lemma (u:unit { (Seq_forall p
-s /\ p x) ==> Seq_forall p (snoc s x)}) *)
-
-(* TODO, ~ TLSInfo.siId; a bit awkward with null_Id *)
-let epoch_id (#region:rid) (#peer:rid) (o: option (epoch region peer)) =
-  match o with 
-  | Some e -> hs_id e.h
-  | None   -> noId
-
-val reader_epoch: #region:rid -> #peer:rid -> e:epoch region peer -> Tot (reader (hs_id e.h))
-let reader_epoch #region #peer (Epoch h r w) = r
-
-val writer_epoch: #region:rid -> #peer:rid -> e:epoch region peer -> Tot (writer (hs_id e.h))
-let writer_epoch #region #peer (Epoch h r w) = w
-
-type epoch_inv (#region:rid) (#peer:rid) (h:HyperHeap.t) (e: epoch region peer) = 
-  st_dec_inv (reader_epoch e) h 
-  /\ st_enc_inv (writer_epoch e) h
-  
-type epochs_inv c h = 
-  Seq_forall (epoch_inv h) (sel h c.hs.log)
-  /\ Map.contains h (HS.region c.hs)
-  /\ Map.contains h (HS.peer c.hs)
-
-//type epochs_inv2 c h = 
-//  Seq_forall (fun e -> epoch_inv e h)
-//             (sel h  (HS.log (C.hs c)))
-
-type st_inv c h = 
-  hs_inv (C.hs c) h /\
-  epochs_inv c h 
-
-val test_st_inv: c:connection -> j:nat -> ST (epoch (HS.region c.hs) (HS.peer c.hs))
-  (requires (fun h -> st_inv c h /\ j < Seq.length (sel h (HS.log c.hs))))
-  (ensures (fun h0 e h1 -> 
-    h0 == h1 /\ 
-    epochs_inv c h1 /\
-    st_dec_inv (reader_epoch e) h1 /\ st_enc_inv (writer_epoch e) h1))
-
-let test_st_inv c j = 
-  let epochs = !c.hs.log in
-  Seq.index epochs j
-
-// we should have st_env_inv & st_dec_inv for all epochs, all the time. 
-// + the property that at most the current epochs' logs are extended.
-val epochs : c:connection -> h:HyperHeap.t -> GTot (es:seq (epoch (HS.region c.hs) (HS.peer c.hs)){epochs_footprint es /\ es = HyperHeap.sel h c.hs.log})
-
-//val epochs : c:connection -> h:HyperHeap.t -> GTot (Handshake.epochs (HS.region c.hs) (HS.peer c.hs))
-let epochs c h = sel h (HS.log c.hs)
-
-
-val frame_epochs: c:connection -> h0:HyperHeap.t -> h1:HyperHeap.t -> Lemma
-  (requires (Map.contains h0 (HS.region c.hs)
-             /\ equal_on (Set.union (Set.singleton (HS.region c.hs))
-      				 (Set.singleton (HS.peer c.hs))) h0 h1))
-  (ensures (epochs c h0 = epochs c h1))
-let frame_epochs c h0 h1 = ()
-
-let epoch_i c h i = Seq.index (epochs c h) i
-
-(** should go to Handshake *)
-
-(* 
-   Aiming to prove that sending a message preserves the 
-   invariant for all the epochs in a connection.
-
-   A connection c encapsulates the state machine of a connection. 
-   It contains within an hs, the handshake state machine. 
-
-   The hs.log field is a ref to a seq of epochs all residing in
-   regions with the same parent region. 
-
-   Each epoch is an (h, r, w) triple, 
-     where the r:StatefulLHAE.reader 
-               w:StatefulLHAE.writer 
-     are each one end of a key pair (their peers are in a some other connection).
-     
-     The h field is the state of the handshake state machine and is
-     irrelevant for this framing lemma.
-
-   In the lemma below, we modify the writer of epoch j
-   and aim to show that the invariant of some arbitrary k is preserved.
-   
-   Later, we generalize over k, using the ghost_lemma combinator to introduce the quantifier.
-*) 
-
-val equal_on_disjoint: s1:set rid -> s2:set rid{disjoint_regions s1 s2} -> r:rid{mem r s1} -> h0:t -> h1:t{modifies (Set.singleton r) h0 h1} -> Lemma (equal_on s2 h0 h1)
-let equal_on_disjoint s1 s2 r h0 h1 = ()
-
-//Move this to the library 
-val ghost_lemma2: #a:Type -> #b:Type -> #p:(a -> b -> Type) -> #q:(a -> b -> unit -> Type) 
-		       -> =f:(x:a -> y:b -> Ghost unit (p x y) (q x y)) 
-		       -> Lemma (forall (x:a) (y:b). p x y ==> q x y ())
-let ghost_lemma2 (#a:Type) (#b:Type) (#p:(a -> b -> Type)) (#q:(a -> b -> unit -> Type)) f = 
-  let f : x:a -> Lemma (forall (y:b). (p x y ==> q x y ())) = 
-    fun x -> ghost_lemma (f x) in
-  qintro f
-  
-val frame_writer_epoch_k: c:connection -> h0:HyperHeap.t -> h1:HyperHeap.t -> j:nat -> k:nat -> Ghost unit 
-  (requires
-    epochs_inv c h0 /\
-    (let es = epochs c h0 in
-     let hs_r = HS.region c.hs in 
-      Map.contains h0 hs_r
-      /\ k < Seq.length es
-      /\ j < Seq.length es 
-      /\ (let wr_j = writer_epoch (Seq.index es j) in
-           modifies (Set.singleton (region wr_j)) h0 h1 
-         /\ st_enc_inv wr_j h1)))
-  (ensures (fun _ -> 
-                epochs c h0 = epochs c h1
-              /\ k < Seq.length (epochs c h1)
-              /\ epoch_inv h1 (epoch_i c h1 k)))
-let frame_writer_epoch_k c h0 h1 j k =
-  let es = epochs c h0 in
-  let hs_r = HS.region c.hs in
-  let e_j = Seq.index es j in
-  let e_k = Seq.index es k in
-  let wr_j = writer_epoch e_j in
-  if k<>j
-  then (equal_on_disjoint (regions e_j) (regions e_k) (region wr_j) h0 h1;
-        frame_st_enc_inv (writer_epoch e_k) h0 h1;
-        frame_st_dec_inv (reader_epoch e_k) h0 h1)
-  else (let r_k = reader_epoch e_k in
-        equal_on_disjoint (regions_of wr_j) (regions_of r_k) (region wr_j) h0 h1;
-        frame_st_dec_inv r_k h0 h1)
-
-opaque type witness (#a:Type) (x:a) = True
-val frame_writer_epoch: c:connection -> h0:HyperHeap.t -> h1:HyperHeap.t -> Lemma 
-  (requires
-    epochs_inv c h0 /\
-    (exists (j:nat). {:pattern (witness j)}
-      (let es = epochs c h0 in
-       let hs_r = HS.region c.hs in 
-       Map.contains h0 hs_r
-       /\ j < Seq.length es 
-       /\ (let wr_j = writer_epoch (Seq.index es j) in
-           modifies (Set.singleton (region wr_j)) h0 h1 
-          /\ st_enc_inv wr_j h1))))
-  (ensures (epochs c h0 = epochs c h1
-            /\ epochs_inv c h1))
-let frame_writer_epoch c h0 h1 = ghost_lemma2 (frame_writer_epoch_k c h0 h1)            
-
-val frame_reader_epoch_k: c:connection -> h0:HyperHeap.t -> h1:HyperHeap.t -> j:nat -> k:nat -> Ghost unit 
-  (requires
-    epochs_inv c h0 /\
-    (let es = epochs c h0 in
-     let hs_r = HS.region c.hs in 
-      Map.contains h0 hs_r
-      /\ k < Seq.length es
-      /\ j < Seq.length es 
-      /\ (let rd_j = reader_epoch (Seq.index es j) in
-           modifies (Set.singleton (region rd_j)) h0 h1 
-         /\ st_dec_inv rd_j h1)))
-  (ensures (fun _ -> 
-                epochs c h0 = epochs c h1
-              /\ k < Seq.length (epochs c h1)
-              /\ epoch_inv h1 (epoch_i c h1 k)))
-let frame_reader_epoch_k c h0 h1 j k =
-  let es = epochs c h0 in
-  let hs_r = HS.region c.hs in
-  let e_j = Seq.index es j in
-  let e_k = Seq.index es k in
-  let rd_j = reader_epoch e_j in
-  if k<>j
-  then (equal_on_disjoint (regions e_j) (regions e_k) (region rd_j) h0 h1;
-        frame_st_enc_inv (writer_epoch e_k) h0 h1;
-        frame_st_dec_inv (reader_epoch e_k) h0 h1)
-  else (let w_k = writer_epoch e_k in
-        equal_on_disjoint (regions_of rd_j) (regions_of w_k) (region rd_j) h0 h1;
-        frame_st_enc_inv w_k h0 h1)
-
-val frame_reader_epoch: c:connection -> h0:HyperHeap.t -> h1:HyperHeap.t -> Lemma 
-  (requires
-    epochs_inv c h0 /\
-    (exists (j:nat).{:pattern (witness j)}
-     (let es = epochs c h0 in
-      let hs_r = HS.region c.hs in 
-      Map.contains h0 hs_r
-      /\ j < Seq.length es 
-      /\ (let rd_j = reader_epoch (Seq.index es j) in
-           modifies (Set.singleton (region rd_j)) h0 h1 
-         /\ st_dec_inv rd_j h1))))
-  (ensures (epochs c h0 = epochs c h1
-            /\ epochs_inv c h1))
-let frame_reader_epoch c h0 h1 = ghost_lemma2 (frame_reader_epoch_k c h0 h1)            
-
-val frame_unrelated_k: c:connection -> h0:HyperHeap.t -> h1:HyperHeap.t -> k:nat -> Ghost unit
-  (requires (epochs_inv c h0 
-	    /\ k < Seq.length (epochs c h0)
-	    /\ equal_on (Set.union (Set.singleton (HS.region c.hs))
-				  (Set.singleton (HS.peer c.hs))) h0 h1))
-  (ensures (fun _ -> 
-	      epochs c h0 = epochs c h1 
-	    /\ k < Seq.length (epochs c h1)
-	    /\ epoch_inv h1 (epoch_i c h1 k)))
-let frame_unrelated_k c h0 h1 k =
-  frame_epochs c h0 h1;
-  let ek = Seq.index (epochs c h0) k in 
-  frame_st_dec_inv (reader_epoch ek) h0 h1;
-  frame_st_enc_inv (writer_epoch ek) h0 h1
-
-val frame_unrelated: c:connection -> h0:HyperHeap.t -> h1:HyperHeap.t -> Lemma
-  (requires (epochs_inv c h0 
-	    /\ equal_on (Set.union (Set.singleton (HS.region c.hs))
-				  (Set.singleton (HS.peer c.hs))) h0 h1))
-  (ensures (epochs c h0 = epochs c h1 
-	    /\ epochs_inv c h1))
-let frame_unrelated c h0 h1 = 
-  ghost_lemma (frame_unrelated_k c h0 h1);
-  frame_epochs c h0 h1
-
 (*
 (* a trivial variant as nothing gets modified; still no trivial proof... *) 
 assume val frame_unmodified: c:connection -> h0:HyperHeap.t -> h1:HyperHeap.t -> Lemma 
@@ -496,7 +240,7 @@ let moveToOpenState c =
     let h0 = ST.get() in
     C.reading c := Open;
     C.writing c := Open;
-    frame_admit c h0 (ST.get())
+    frame_unrelated c h0 (ST.get())
 
 
 assume val epoch_pv: #region:rid -> #peer:rid -> epoch region peer -> Tot ProtocolVersion
@@ -536,12 +280,13 @@ val closeConnection: c: connection -> ST unit
 
 let closeConnection c =
     let h0 = ST.get() in
-    invalidateSession (C.hs c);
+    recall (HS.log c.hs); 
+    recall (HS.state c.hs); // needed to preserve hs_inv within inv
+    invalidateSession c.hs; //changes (HS.region c.hs)
     let h1 = ST.get() in 
-    recall (HS.log c.hs); recall (HS.state c.hs); // needed to preserve hs_inv within inv
     c.reading := Closed;
     c.writing := Closed;
-    frame_admit c h0 (ST.get()) 
+    frame_admit c h0 (ST.get()) //NS: TODO: not quite an application of frame_unrelated; since invalidate
 
 // on some errors, we locally give up the connection
 let unrecoverable c reason =
@@ -557,13 +302,13 @@ val abortWithAlert: c:connection -> ad:alertDescription{isFatal ad} -> reason:st
 let abortWithAlert c ad reason =
     let closingPV = pickSendPV c in
     let h0 = ST.get() in
-    invalidateSession c.hs;
+    invalidateSession c.hs;    
     frame_admit c h0 (ST.get());
     let h0 = ST.get() in
     Alert.send c.alert ad;
     c.reading := Closed;
     c.writing := Closing(closingPV,reason);
-    frame_admit c h0 (ST.get())
+    frame_admit c h0 (ST.get()) //NS: again, not an instance of frame_unrelated, because of invalidateSession
 
 // on some errors, we attempt to send an alert before tearing down the connection
 let closable c reason =
@@ -737,7 +482,7 @@ let send c i f =
   //15-11-27 st_inv c h1 across this call; what's a better style?
   let h0 = ST.get() in 
   let r = Platform.Tcp.send (C.tcp c) record in
-  frame_unrelated c h0 (ST.get());//  frame_admit c h0 (ST.get());
+  frame_unrelated c h0 (ST.get());
   match r with
     | Error(x)  -> Error(AD_internal_error,x)
     | Correct _ -> Correct()
@@ -809,9 +554,9 @@ let writeOne c i appdata =
       | Some(Epoch h _ w) -> recall (log w); recall (seqn w));
   
       let h0 = ST.get() in
-      let alert_response = Alert.next_fragment (C.alert c) in 
+      let alert_response = Alert.next_fragment c.alert in 
       let h1 = ST.get() in 
-      frame_admit c h0 h1;
+      frame_admit c h0 h1; //NS: not an instance of frame_unrelated ... next_fragment changes c.hs.region
       match alert_response with // alerts have highest priority
       | Some AD_close_notify ->
           ( match writing  with
@@ -821,7 +566,11 @@ let writeOne c i appdata =
                If we already received the other close notify, then reading is already closed,
                otherwise we wait to read it, then close. But do not close here. *)
               ( match send c #i (Content.ct_alert i AD_close_notify) with
-                | Correct()   -> c.writing := Closed; frame_admit c h1 (ST.get()); SentClose //FIXME
+                | Correct()   -> 
+		  let h2 = ST.get () in 
+		  c.writing := Closed; 
+		  frame_unrelated c h2 (ST.get()); 
+		  SentClose //FIXME
                 | Error (x,y) -> unrecoverable c y)
             | _ -> unrecoverable c (perror __SOURCE_FILE__ __LINE__ "Sending alert message in wrong state"))
       | Some ad ->
@@ -838,7 +587,7 @@ let writeOne c i appdata =
       | None ->
           ( let hs_response = Handshake.next_fragment c.hs in
             let h2 = ST.get() in 
-            frame_admit c h1 h2;
+            frame_admit c h1 h2; //NS: not an instance of frame_unrelated ... next_fragment changes c.hs.region
             match hs_response with // next we check if there are outgoing Handshake messages
             | Handshake.OutCCS -> (* send a (complete) CCS fragment *)
                 ( match writing with
@@ -873,8 +622,12 @@ let writeOne c i appdata =
                 ( match writing with
                   | Finishing ->
                       ( match send c #i (Content.CT_Handshake rg last_fragment) with
-                        | Correct()   -> c.writing := Finished; frame_admit c h2 (ST.get()); WriteAgain (* TODO 15-09-11 recheck, was WriteFinished *)
-                                                                          (* also move to the Finished state *)
+                        | Correct()   -> 
+			  let h3 = ST.get () in
+			  c.writing := Finished; 
+			  frame_unrelated c h3 (ST.get()); 
+			  WriteAgain (* TODO 15-09-11 recheck, was WriteFinished *)
+                                     (* also move to the Finished state *)
                         | Error (x,y) -> unrecoverable c y)
                   | _ -> closable c (perror __SOURCE_FILE__ __LINE__ "Sending handshake message in wrong state"))
 
