src/tls/Connection.fst
@@ -1,0 +1,277 @@
+module Connection
+
+// 2015-08-25 largely rewritten to implement both stateful dispatch and TLS
+
+open FStar.Heap
+open FStar.HyperHeap
+open FStar.Seq
+open FStar.SeqProperties // for e.g. found
+open FStar.Set
+ 
+open Platform.Bytes
+open Platform.Error
+open Platform.Tcp
+
+open TLSError
+open TLSConstants
+open TLSInfo
+
+open Range
+open StatefulLHAE // via its interface
+open Handshake    // via its interface
+
+// using also Alert, Range, DataStream, TLSFragment, Record
+
+// internal state machine (one for reading, one for writing; a bit much)
+// TODO make it private?
+// TODO write invariant, to cut out cases in code
+// e.g. , reading, and writing transitions are tighly related
+// TODO recheck large logical invariants GState in Dispatch.fs7
+
+// private //TODO: restore this qualifier; NS:commenting for now
+type dispatch =
+  | Init
+  | FirstHandshake of ProtocolVersion (* bound by ServerHello *)
+  | Finishing
+  | Finished
+  | Open
+  | Closing of ProtocolVersion * string (* write-only, while sending a fatal alert *)
+  | Closed
+ 
+type connection = | C:
+  #region: rid ->
+  peer:   rid{disjoint region peer} ->
+  hs:      hs { extends (HS.region hs) region /\ extends (HS.peer hs) peer } (* providing role, config, and uid *) ->
+  alert:   Alert.state  { extends (Alert.State.region alert) region /\ HS.region hs <> Alert.State.region alert } (* review *) ->
+  tcp:     networkStream ->
+  reading: rref region dispatch ->
+  writing: rref region dispatch ->
+  connection
+
+let c_role c   = c.hs.r
+let c_id c     = c.hs.id
+let c_cfg c    = c.hs.cfg
+let c_resume c = c.hs.resume
+let c_log c    = c.hs.log
+
+
+(*** top-level invariant (TBC) ***) 
+
+// we'll rely on the invariant to show we picked the correct index
+
+opaque type Seq_forall (#a:Type) (p: a -> Type) (s:seq a) =
+  forall (j: nat { j < Seq.length s }).{:pattern (Seq.index s j)} p (Seq.index s j)
+
+let test_1 (p:nat -> Type) (s:seq nat { Seq_forall p s }) = assert(p 12 ==> Seq_forall p (snoc s 12))
+let test_2 (p:nat -> Type) (s:seq nat { Seq_forall p s }) (j:nat { j < Seq.length s }) =  let x = Seq.index s j in assert(p x)
+//let test_3 (p:nat -> Type) (s:seq nat { Seq_forall p s }) x = assert(SeqProperties.mem x s ==> p x)
+
+
+(* usage? how to prove this lemma?  val exercise_seq_forall: #a:Type
+-> p: (a -> Type) -> s:seq a -> x: a -> Lemma (u:unit { (Seq_forall p
+s /\ p x) ==> Seq_forall p (snoc s x)}) *)
+
+(* TODO, ~ TLSInfo.siId; a bit awkward with null_Id *)
+let epoch_id (#region:rid) (#peer:rid) (o: option (epoch region peer)) =
+  match o with 
+  | Some e -> hs_id e.h
+  | None   -> noId
+
+val reader_epoch: #region:rid -> #peer:rid -> e:epoch region peer -> Tot (reader (hs_id e.h))
+let reader_epoch #region #peer (Epoch h r w) = r
+
+val writer_epoch: #region:rid -> #peer:rid -> e:epoch region peer -> Tot (writer (hs_id e.h))
+let writer_epoch #region #peer (Epoch h r w) = w
+
+type epoch_inv (#region:rid) (#peer:rid) (h:HyperHeap.t) (e: epoch region peer) = 
+  st_dec_inv (reader_epoch e) h 
+  /\ st_enc_inv (writer_epoch e) h
+  
+type epochs_inv c h = 
+  Seq_forall (epoch_inv h) (sel h c.hs.log)
+  /\ Map.contains h (HS.region c.hs)
+  /\ Map.contains h (HS.peer c.hs)
+
+type st_inv c h = 
+  hs_inv (C.hs c) h /\
+  epochs_inv c h 
+
+val test_st_inv: c:connection -> j:nat -> ST (epoch (HS.region c.hs) (HS.peer c.hs))
+  (requires (fun h -> st_inv c h /\ j < Seq.length (sel h (HS.log c.hs))))
+  (ensures (fun h0 e h1 -> 
+    h0 == h1 /\ 
+    epochs_inv c h1 /\
+    st_dec_inv (reader_epoch e) h1 /\ st_enc_inv (writer_epoch e) h1))
+
+let test_st_inv c j = 
+  let epochs = !c.hs.log in
+  Seq.index epochs j
+
+// we should have st_env_inv & st_dec_inv for all epochs, all the time. 
+// + the property that at most the current epochs' logs are extended.
+val epochs : c:connection -> h:HyperHeap.t -> GTot (es:seq (epoch (HS.region c.hs) (HS.peer c.hs)){epochs_footprint es /\ es = HyperHeap.sel h c.hs.log})
+
+//val epochs : c:connection -> h:HyperHeap.t -> GTot (Handshake.epochs (HS.region c.hs) (HS.peer c.hs))
+let epochs c h = sel h (HS.log c.hs)
+
+
+val frame_epochs: c:connection -> h0:HyperHeap.t -> h1:HyperHeap.t -> Lemma
+  (requires (Map.contains h0 (HS.region c.hs)
+             /\ equal_on (Set.union (Set.singleton (HS.region c.hs))
+      				 (Set.singleton (HS.peer c.hs))) h0 h1))
+  (ensures (epochs c h0 = epochs c h1))
+let frame_epochs c h0 h1 = ()
+
+let epoch_i c h i = Seq.index (epochs c h) i
+
+(** should go to Handshake *)
+
+(* 
+   Aiming to prove that sending a message preserves the 
+   invariant for all the epochs in a connection.
+
+   A connection c encapsulates the state machine of a connection. 
+   It contains within an hs, the handshake state machine. 
+
+   The hs.log field is a ref to a seq of epochs all residing in
+   regions with the same parent region. 
+
+   Each epoch is an (h, r, w) triple, 
+     where the r:StatefulLHAE.reader 
+               w:StatefulLHAE.writer 
+     are each one end of a key pair (their peers are in a some other connection).
+     
+     The h field is the state of the handshake state machine and is
+     irrelevant for this framing lemma.
+
+   In the lemma below, we modify the writer of epoch j
+   and aim to show that the invariant of some arbitrary k is preserved.
+   
+   Later, we generalize over k, using the ghost_lemma combinator to introduce the quantifier.
+*) 
+
+val equal_on_disjoint: s1:set rid -> s2:set rid{disjoint_regions s1 s2} -> r:rid{mem r s1} -> h0:t -> h1:t{modifies (Set.singleton r) h0 h1} -> Lemma (equal_on s2 h0 h1)
+let equal_on_disjoint s1 s2 r h0 h1 = ()
+
+//Move this to the library 
+val ghost_lemma2: #a:Type -> #b:Type -> #p:(a -> b -> Type) -> #q:(a -> b -> unit -> Type) 
+		       -> =f:(x:a -> y:b -> Ghost unit (p x y) (q x y)) 
+		       -> Lemma (forall (x:a) (y:b). p x y ==> q x y ())
+let ghost_lemma2 (#a:Type) (#b:Type) (#p:(a -> b -> Type)) (#q:(a -> b -> unit -> Type)) f = 
+  let f : x:a -> Lemma (forall (y:b). (p x y ==> q x y ())) = 
+    fun x -> ghost_lemma (f x) in
+  qintro f
+  
+val frame_writer_epoch_k: c:connection -> h0:HyperHeap.t -> h1:HyperHeap.t -> j:nat -> k:nat -> Ghost unit 
+  (requires
+    epochs_inv c h0 /\
+    (let es = epochs c h0 in
+     let hs_r = HS.region c.hs in 
+      Map.contains h0 hs_r
+      /\ k < Seq.length es
+      /\ j < Seq.length es 
+      /\ (let wr_j = writer_epoch (Seq.index es j) in
+           modifies (Set.singleton (region wr_j)) h0 h1 
+         /\ st_enc_inv wr_j h1)))
+  (ensures (fun _ -> 
+                epochs c h0 = epochs c h1
+              /\ k < Seq.length (epochs c h1)
+              /\ epoch_inv h1 (epoch_i c h1 k)))
+let frame_writer_epoch_k c h0 h1 j k =
+  let es = epochs c h0 in
+  let hs_r = HS.region c.hs in
+  let e_j = Seq.index es j in
+  let e_k = Seq.index es k in
+  let wr_j = writer_epoch e_j in
+  if k<>j
+  then (equal_on_disjoint (regions e_j) (regions e_k) (region wr_j) h0 h1;
+        frame_st_enc_inv (writer_epoch e_k) h0 h1;
+        frame_st_dec_inv (reader_epoch e_k) h0 h1)
+  else (let r_k = reader_epoch e_k in
+        equal_on_disjoint (regions_of wr_j) (regions_of r_k) (region wr_j) h0 h1;
+        frame_st_dec_inv r_k h0 h1)
+
+opaque type witness (#a:Type) (x:a) = True
+val frame_writer_epoch: c:connection -> h0:HyperHeap.t -> h1:HyperHeap.t -> Lemma 
+  (requires
+    epochs_inv c h0 /\
+    (exists (j:nat). {:pattern (witness j)}
+      (let es = epochs c h0 in
+       let hs_r = HS.region c.hs in 
+       Map.contains h0 hs_r
+       /\ j < Seq.length es 
+       /\ (let wr_j = writer_epoch (Seq.index es j) in
+           modifies (Set.singleton (region wr_j)) h0 h1 
+          /\ st_enc_inv wr_j h1))))
+  (ensures (epochs c h0 = epochs c h1
+            /\ epochs_inv c h1))
+let frame_writer_epoch c h0 h1 = ghost_lemma2 (frame_writer_epoch_k c h0 h1)            
+
+val frame_reader_epoch_k: c:connection -> h0:HyperHeap.t -> h1:HyperHeap.t -> j:nat -> k:nat -> Ghost unit 
+  (requires
+    epochs_inv c h0 /\
+    (let es = epochs c h0 in
+     let hs_r = HS.region c.hs in 
+      Map.contains h0 hs_r
+      /\ k < Seq.length es
+      /\ j < Seq.length es 
+      /\ (let rd_j = reader_epoch (Seq.index es j) in
+           modifies (Set.singleton (region rd_j)) h0 h1 
+         /\ st_dec_inv rd_j h1)))
+  (ensures (fun _ -> 
+                epochs c h0 = epochs c h1
+              /\ k < Seq.length (epochs c h1)
+              /\ epoch_inv h1 (epoch_i c h1 k)))
+let frame_reader_epoch_k c h0 h1 j k =
+  let es = epochs c h0 in
+  let hs_r = HS.region c.hs in
+  let e_j = Seq.index es j in
+  let e_k = Seq.index es k in
+  let rd_j = reader_epoch e_j in
+  if k<>j
+  then (equal_on_disjoint (regions e_j) (regions e_k) (region rd_j) h0 h1;
+        frame_st_enc_inv (writer_epoch e_k) h0 h1;
+        frame_st_dec_inv (reader_epoch e_k) h0 h1)
+  else (let w_k = writer_epoch e_k in
+        equal_on_disjoint (regions_of rd_j) (regions_of w_k) (region rd_j) h0 h1;
+        frame_st_enc_inv w_k h0 h1)
+
+val frame_reader_epoch: c:connection -> h0:HyperHeap.t -> h1:HyperHeap.t -> Lemma 
+  (requires
+    epochs_inv c h0 /\
+    (exists (j:nat).{:pattern (witness j)}
+     (let es = epochs c h0 in
+      let hs_r = HS.region c.hs in 
+      Map.contains h0 hs_r
+      /\ j < Seq.length es 
+      /\ (let rd_j = reader_epoch (Seq.index es j) in
+           modifies (Set.singleton (region rd_j)) h0 h1 
+         /\ st_dec_inv rd_j h1))))
+  (ensures (epochs c h0 = epochs c h1
+            /\ epochs_inv c h1))
+let frame_reader_epoch c h0 h1 = ghost_lemma2 (frame_reader_epoch_k c h0 h1)            
+
+val frame_unrelated_k: c:connection -> h0:HyperHeap.t -> h1:HyperHeap.t -> k:nat -> Ghost unit
+  (requires (epochs_inv c h0 
+	    /\ k < Seq.length (epochs c h0)
+	    /\ equal_on (Set.union (Set.singleton (HS.region c.hs))
+				  (Set.singleton (HS.peer c.hs))) h0 h1))
+  (ensures (fun _ -> 
+	      epochs c h0 = epochs c h1 
+	    /\ k < Seq.length (epochs c h1)
+	    /\ epoch_inv h1 (epoch_i c h1 k)))
+let frame_unrelated_k c h0 h1 k =
+  frame_epochs c h0 h1;
+  let ek = Seq.index (epochs c h0) k in 
+  frame_st_dec_inv (reader_epoch ek) h0 h1;
+  frame_st_enc_inv (writer_epoch ek) h0 h1
+
+val frame_unrelated: c:connection -> h0:HyperHeap.t -> h1:HyperHeap.t -> Lemma
+  (requires (epochs_inv c h0 
+	    /\ equal_on (Set.union (Set.singleton (HS.region c.hs))
+				  (Set.singleton (HS.peer c.hs))) h0 h1))
+  (ensures (epochs c h0 = epochs c h1 
+	    /\ epochs_inv c h1))
+let frame_unrelated c h0 h1 = 
+  ghost_lemma (frame_unrelated_k c h0 h1);
+  frame_epochs c h0 h1
